src/x86/instrrules/callrel.v
@@ -12,11 +12,11 @@ Lemma CALLrel_rule (p q: DWORD) (tgt: JmpTgt) (w sp:DWORD):
       (
       |> safe @ (EIP ~= p' ** P ** ESP~=sp-#4 ** sp-#4 :-> q) -->>
          safe @ (EIP ~= p  ** P ** ESP~=sp    ** sp-#4 :-> w)
-    ) <@ (p -- q :-> CALLrel tgt)).
+    ) @ (p -- q :-> CALLrel tgt)).
 Proof.
   rewrite /interpJmpTgt/interpMemSpecSrc.
   do_instrrule
-    ((try specintros => *; autorewrite with push_at);
+    (try specintros => *;
      apply: TRIPLE_safeLater => ?;
      do !instrrule_triple_bazooka_step idtac).
 Qed.
@@ -29,18 +29,17 @@ Global Instance: forall tgt : JmpTgt, instrrule (CALLrel tgt) := fun tgt p q => 
 Section specapply_hint.
 Local Hint Unfold interpJmpTgt : specapply.
 
-Ltac myspecapply R := (specapply R; last try rewrite <- spec_later_weaken).
 Corollary CALLrel_R_rule (r:Reg) (p q: DWORD) :
   |-- Forall (w sp: DWORD) p', (
       |> safe @ (EIP ~= p' ** r~=p' ** ESP~=sp-#4 ** sp-#4 :-> q) -->>
          safe @ (EIP ~= p  ** r~=p' ** ESP~=sp    ** sp-#4 :-> w)
-    ) <@ (p -- q :-> CALLrel r).
-Proof. specintros => *. myspecapply (@CALLrel_rule p q r); finish_logic_with sbazooka. Qed.
+    ) @ (p -- q :-> CALLrel r).
+Proof. specintros => *. safeapply (@CALLrel_rule p q r); finish_logic_with sbazooka. Qed.
 
 Corollary CALLrel_I_rule (rel: DWORD) (p q: DWORD) :
   |-- Forall (w sp: DWORD), (
       |> safe @ (EIP ~= addB q rel ** ESP~=sp-#4 ** sp-#4 :-> q) -->>
          safe @ (EIP ~= p          ** ESP~=sp    ** sp-#4 :-> w)
-    ) <@ (p -- q :-> CALLrel rel).
-Proof. specintros => *. specapply (@CALLrel_rule p q rel); finish_logic_with sbazooka. Qed.
+    ) @ (p -- q :-> CALLrel rel).
+Proof. specintros => *. safeapply (@CALLrel_rule p q rel); finish_logic_with sbazooka. Qed.
 End specapply_hint.
