src/x86/wrapalloc.v
@@ -27,12 +27,12 @@ Lemma wrappedAlloc_correct bytes (r1 r2: Reg) heapInfo :
   toyfun i EDI? ((Exists p:DWORD, EDI ~= p ** memAny p (p +# bytes)) \\// EDI ~= #0)
 
   @  (ESI? ** OSZCP? ** allocInv heapInfo)
-  <@ (i -- j :-> mkbody_toyfun (wrappedAlloc bytes r1 r2 heapInfo)).
+  @ (i -- j :-> mkbody_toyfun (wrappedAlloc bytes r1 r2 heapInfo)).
 Proof.
 specintros => i j.
 
 (* First deal with the calling-convention wrapper *)
-autorewrite with push_at.
+rewrite spec_at_toyfun.
 etransitivity; [|apply toyfun_mkbody]. specintro => iret.
 
 (* Now unfold the control-flow logic *)
@@ -40,7 +40,10 @@ rewrite /wrappedAlloc/basic. specintros => i1 i2. unfold_program.
 specintros => i3 i4 i5 i6 i7 i8 -> -> i9 -> ->.
 
 (* Deal with the allocator spec itself *)
-specapply inlineAlloc_correct; first by ssimpl.
+have IC := @inlineAlloc_correct bytes.
+rewrite /allocSpec in IC. 
+eforalls IC. rewrite -> spec_at_impl in IC. rewrite -> spec_at_at in IC. 
+safeapply IC; first by ssimpl. 
 
 (* Now we deal with failure and success cases *)
 specsplit.
@@ -48,7 +51,7 @@ specsplit.
 (* failure case *)
 
 (* MOV EDI, 0 *)
-specapply MOV_RanyI_rule; first by ssimpl. 
+safeapply (MOV_RanyI_rule (r:=EDI)); first by ssimpl. 
 finish_logic_with sbazooka. apply: lorR2. by rewrite /natAsDWORD.
 
 (* success case *)
@@ -61,10 +64,10 @@ assert (H:= subB_equiv_addB_negB (pb+#bytes) # bytes).
 rewrite E0 in H. simpl (snd _) in H. rewrite addB_negBn in H.
 rewrite H in E0.
 
-specapply SUB_RI_rule; first by ssimpl. 
+safeapply (SUB_RI_rule (r1:=EDI)); first by ssimpl. 
 
 (* JMP SUCCEED *)
-specapply JMP_I_rule; first by ssimpl.
+safeapply JMP_I_rule; first by ssimpl.
 rewrite <- spec_later_weaken. 
 
 (* Final stuff *)
